theories/type_systems/systemf_state/deterministic.v
@@ -1,0 +1,86 @@
+From stdpp Require Import gmap base relations.
+From ffpl.lib Require Import prelude.
+From ffpl.type_systems.systemf_state Require Import lang notation.
+From Equations Require Import Equations.
+
+(** Proof that our small-step semantics are deterministic. *)
+
+Lemma base_step_det h e h1 e1 h2 e2 :
+  base_step (h, e) (h1, e1) -> base_step (h, e) (h2, e2) -> h1 = h2 /\ e1 = e2.
+Proof.
+  inversion 1; inversion 1; subst; split; congruence.
+Qed.
+
+(** We need this very technical lemma with tons of cases. None of the cases is
+very interesting. We use some Coq tactic programming to handle them all
+automatically. *)
+
+Lemma base_redex_unique K1 h e1 h1' e1' K2 e2 h2' e2' :
+  fill K1 e1 = fill K2 e2 ->
+  base_step (h, e1) (h1', e1') ->
+  base_step (h, e2) (h2', e2') ->
+  K1 = K2 /\ e1 = e2.
+Proof.
+  induction K1 in K2, e2, e2' |- *; simpl.
+  all: destruct K2; intros; simplify_eq/=.
+  all: repeat match goal with
+      | H : ?e' = fill ?K ?e |- _ =>
+          (* maybe [e'] is a value *)
+          let Hval := fresh "Hval" in
+          assert (is_val e') as Hval by (by eauto);
+          rewrite H in Hval;
+          clear H (* avoid loops *)
+      | H : fill ?K ?e = of_val _ |- _ =>
+          symmetry in H (* make it hit the case above *)
+      | H : is_val (fill _ _) |- _ =>
+          apply fill_is_val_inv in H
+      | H : to_val (fill _ _) = Some _ |- _ =>
+          apply is_val_to_val in H
+      | H1 : is_val ?e, H2 : base_step (_, ?e) _ |- _ =>
+          apply base_step_no_val in H2; done
+      | H : fill _ ?e1 = fill _ ?e2, H1 : base_step (_, ?e1) _, H2 : base_step (_, ?e2) _ |- _ =>
+          destruct (IHK1 _ _ _ H H1 H2); simplify_eq/=; by eauto
+      | H : base_step _ _ |- _ =>
+          inversion H;
+          simplify_eq/=;
+          [clear H] (* also asserts that there is exactly one goal *)
+      | H : base_step _ _ |- _ =>
+          inversion H;
+          simplify_eq/=;
+          done (* sometimes this closes all goals *)
+      | H : base_step _ _ |- _ =>
+          inversion H;
+          simplify_eq/=;
+          [clear H|clear H] (* for if, we need to allow 2 goals *)
+      end.
+Qed.
+
+Lemma contextual_step_det {h e h1 e1 h2 e2} :
+  contextual_step (h, e) (h1, e1) -> contextual_step (h, e) (h2, e2) -> h1 = h2 /\ e1 = e2.
+Proof.
+  inversion 1; inversion 1; subst.
+  edestruct base_redex_unique; [done|done|done|subst]. split.
+  - eapply base_step_det; done.
+  - f_equal. eapply base_step_det; done.
+Qed.
+
+(** It follows that if [e] can step to two different terms, then
+really one is just a more reduced form of the other. *)
+Lemma contextual_steps_det {h e h1 e1 h2 e2} :
+  rtc contextual_step (h, e) (h1, e1) ->
+  rtc contextual_step (h, e) (h2, e2) ->
+  (rtc contextual_step (h1, e1) (h2, e2) \/ rtc contextual_step (h2, e2) (h1, e1)).
+Proof.
+  remember (h, e) as cfg.
+  remember (h1, e1) as cfg1.
+  remember (h2, e2) as cfg2.
+  induction 1 as [cfg|cfg cfg1' cfg1 Hstep1 Hsteps1 IH] in h, e, Heqcfg, h1, h2, Heqcfg1, h2, e2, cfg2, Heqcfg2 |- *.
+  { simplify_eq/=. eauto. }
+  destruct 1 as [cfg|cfg cfg2' cfg2 Hstep2 Hsteps2].
+  { simplify_eq/=. right. econstructor; done. }
+  destruct cfg1' as [h1' e1'].
+  destruct cfg2' as [h2' e2'].
+  simplify_eq/=.
+  pose proof (contextual_step_det Hstep1 Hstep2) as [-> ->].
+  eapply IH; done.
+Qed.
