theories/type_systems/systemf_state/types.v
@@ -1,0 +1,944 @@
+From stdpp Require Import base relations.
+From ffpl.lib Require Import prelude.
+From ffpl.lib Require Import maps.
+From ffpl.type_systems.systemf_state Require Import lang notation.
+From Autosubst Require Export Autosubst.
+
+(** ** Syntactic typing *)
+(** We use De Bruijn indices with the help of the Autosubst library. *)
+Inductive type : Type :=
+  (** [var] is the type of variables of Autosubst -- it unfolds to [nat] *)
+  | TVar : var -> type
+  | Int
+  | Bool
+  | Unit
+  (** The [{bind 1 of type}] tells Autosubst to put a De Bruijn binder here *)
+  | TForall : {bind 1 of type} -> type
+  | TExists : {bind 1 of type} -> type
+  | Fun (A B : type)
+  | Prod (A B : type)
+  | Ref (A : type)
+.
+
+(** Autosubst instances.
+  This lets Autosubst do its magic and derive all the substitution functions, etc.
+ *)
+#[export] Instance Ids_type : Ids type. derive. Defined.
+#[export] Instance Rename_type : Rename type. derive. Defined.
+#[export] Instance Subst_type : Subst type. derive. Defined.
+#[export] Instance SubstLemmas_typer : SubstLemmas type. derive. Qed.
+
+Notation typing_context := (list type).
+Notation typevar_context := nat.
+Notation heap_context := (gmap loc type).
+
+Implicit Types
+  (Sigma : heap_context)
+  (Delta : typevar_context)
+  (Gamma : typing_context)
+  (v : val)
+  (e : expr).
+
+Declare Scope FType_scope.
+Delimit Scope FType_scope with ty.
+Bind Scope FType_scope with type.
+Notation "^ x" := (TVar x) : FType_scope.
+Infix "->" := Fun : FType_scope.
+Notation "(->)" := Fun (only parsing) : FType_scope.
+Notation "forall: tau" :=
+  (TForall tau%ty)
+  (at level 100, tau at level 200) : FType_scope.
+Notation "exists: tau" :=
+  (TExists tau%ty)
+  (at level 100, tau at level 200) : FType_scope.
+Infix "*" := Prod : FType_scope.
+Notation "(\*)" := Prod (only parsing) : FType_scope.
+
+(** Shift all the indices in the context by one,
+   used when a new type variable is introduced. *)
+(* [<$>] is notation for the [fmap] operation that maps the substitution over the whole map. *)
+(* [ren] is Autosubst's renaming operation -- it renames all type variables according to the given function,
+  in this case [S] to shift the variables up by 1. *)
+Definition upctx Gamma := subst (ren S) <$> Gamma.
+Definition upheap Sigma := subst (ren S) <$> Sigma.
+
+(** [type_wf Delta A] states that a type [A] has only free variables in [Delta].
+ (in other words, all variables occurring free are strictly bounded by [Delta]). *)
+Inductive type_wf : typevar_context -> type -> Prop :=
+  | type_wf_TVar alpha Delta :
+      alpha < Delta ->
+      type_wf Delta (TVar alpha)
+  | type_wf_Int Delta : type_wf Delta Int
+  | type_wf_Bool Delta : type_wf Delta Bool
+  | type_wf_Unit Delta : type_wf Delta Unit
+  | type_wf_TForall Delta A :
+      type_wf (S Delta) A ->
+      type_wf Delta (TForall A)
+  | type_wf_TExists Delta A :
+      type_wf (S Delta) A ->
+      type_wf Delta (TExists A)
+  | type_wf_Fun Delta A B :
+      type_wf Delta A ->
+      type_wf Delta B ->
+      type_wf Delta (Fun A B)
+  | type_wf_Prod Delta A B :
+      type_wf Delta A ->
+      type_wf Delta B ->
+      type_wf Delta (Prod A B)
+  | type_wf_ref n A :
+      type_wf n A ->
+      type_wf n (Ref A)
+.
+#[export] Hint Constructors type_wf : core.
+
+Inductive bin_op_typed : bin_op -> type -> type -> type -> Prop :=
+  | plus_op_typed : bin_op_typed PlusOp Int Int Int
+  | minus_op_typed : bin_op_typed MinusOp Int Int Int
+  | mul_op_typed : bin_op_typed MultOp Int Int Int
+  | lt_op_typed : bin_op_typed LtOp Int Int Bool
+  | le_op_typed : bin_op_typed LeOp Int Int Bool
+  | eq_op_typed : bin_op_typed EqOp Int Int Bool.
+#[export] Hint Constructors bin_op_typed : core.
+
+Reserved Notation "'TY' Sigma ; Delta ; Gamma |- e : A" (at level 74, e, A at next level).
+Inductive syn_typed : heap_context -> typevar_context -> typing_context -> expr -> type -> Prop :=
+  | type_var Sigma Delta Gamma x A :
+      Gamma !! x = Some A ->
+      TY Sigma; Delta; Gamma |- (Var x) : A
+  | type_lam Sigma Delta Gamma e A B :
+      TY Sigma; Delta ; (A :: Gamma) |- e : B ->
+      type_wf Delta A ->
+      TY Sigma; Delta; Gamma |- (Lam e) : (A -> B)
+  | type_app Sigma Delta Gamma e1 e2 A B :
+      TY Sigma; Delta; Gamma |- e1 : (A -> B) ->
+      TY Sigma; Delta; Gamma |- e2 : A ->
+      TY Sigma; Delta; Gamma |- (e1 e2)%E : B
+  | type_tlam Sigma Delta Gamma e A :
+      (* we need to shift the context up as we descend under a binder *)
+      TY (upheap Sigma); (S Delta); (upctx Gamma) |- e : A ->
+      TY Sigma; Delta; Gamma |- (Lam: e) : (forall: A)
+  | type_tapp Sigma Delta Gamma A B e :
+      TY Sigma; Delta; Gamma |- e : (forall: A) ->
+      type_wf Delta B ->
+      (* A.[B/] is the notation for Autosubst's substitution operation that
+        replaces variable 0 by [B] *)
+      TY Sigma; Delta; Gamma |- (e <>) : (A.[B/])
+  | type_pack Sigma Delta Gamma A B e :
+      type_wf Delta B ->
+      TY Sigma; Delta; Gamma |- e : (A.[B/]) ->
+      TY Sigma; Delta; Gamma |- (pack e) : (exists: A)
+  | type_unpack Sigma Delta Gamma A B e e' :
+      type_wf Delta B -> (* we should not leak the existential! *)
+      TY Sigma; Delta; Gamma |- e : (exists: A) ->
+      (* As we descend under a type variable binder for the typing of [e'],
+          we need to shift the indices in [Gamma] and [B] up by one.
+        On the other hand, [A] is already defined under this binder, so we need not shift it.
+      *)
+      TY upheap Sigma; (S Delta); (A :: (upctx Gamma)) |- e' : (B.[ren (+1)]) ->
+      TY Sigma; Delta; Gamma |- (unpack e in e') : B
+  | type_int Sigma Delta Gamma z :
+      TY Sigma; Delta; Gamma |- (Lit $ LitInt z) : Int
+  | type_bool Sigma Delta Gamma b :
+      TY Sigma; Delta; Gamma |- (Lit $ LitBool b) : Bool
+  | type_unit Sigma Delta Gamma :
+      TY Sigma; Delta; Gamma |- (Lit $ LitUnit) : Unit
+  | type_if Sigma Delta Gamma e0 e1 e2 A :
+      TY Sigma; Delta; Gamma |- e0 : Bool ->
+      TY Sigma; Delta; Gamma |- e1 : A ->
+      TY Sigma; Delta; Gamma |- e2 : A ->
+      TY Sigma; Delta; Gamma |- If e0 e1 e2 : A
+  | type_binop Sigma Delta Gamma e1 e2 op A B C :
+      bin_op_typed op A B C ->
+      TY Sigma; Delta; Gamma |- e1 : A ->
+      TY Sigma; Delta; Gamma |- e2 : B ->
+      TY Sigma; Delta; Gamma |- BinOp op e1 e2 : C
+  | type_pair Sigma Delta Gamma e1 e2 A B :
+      TY Sigma; Delta; Gamma |- e1 : A ->
+      TY Sigma; Delta; Gamma |- e2 : B ->
+      TY Sigma; Delta; Gamma |- (e1, e2) : A * B
+  | type_fst Sigma Delta Gamma e A B :
+      TY Sigma; Delta; Gamma |- e : A * B ->
+      TY Sigma; Delta; Gamma |- Fst e : A
+  | type_snd Sigma Delta Gamma e A B :
+      TY Sigma; Delta; Gamma |- e : A * B ->
+      TY Sigma; Delta; Gamma |- Snd e : B
+  | type_loc Sigma Delta Gamma l A :
+      Sigma !! l = Some A ->
+      TY Sigma; Delta; Gamma |- (Lit $ LitLoc l) : (Ref A)
+  | type_load Sigma Delta Gamma e A :
+      TY Sigma; Delta; Gamma |- e : (Ref A) ->
+      TY Sigma; Delta; Gamma |- !e : A
+  | type_store Sigma Delta Gamma e1 e2 A :
+      TY Sigma; Delta; Gamma |- e1 : (Ref A) ->
+      TY Sigma; Delta; Gamma |- e2 : A ->
+      TY Sigma; Delta; Gamma |- (e1 <- e2) : A
+  | type_new Sigma Delta Gamma e A :
+      TY Sigma; Delta; Gamma |- e : A ->
+      TY Sigma; Delta; Gamma |- (new e) : Ref A
+where "'TY' Sigma ; Delta ; Gamma |- e : A" := (syn_typed Sigma Delta Gamma e%E A%ty).
+#[export] Hint Constructors syn_typed : core.
+
+(** A heap is well-typed in [Sigma] if, for all entries in [Sigma],
+the heap contains some (closed) value [v] of the right type. *)
+Definition typed_heap Sigma (h : heap) :=
+  forall l A, Sigma !! l = Some A ->
+    exists v, h !! l = Some v /\ TY Sigma; 0; [] |- of_val v : A.
+
+(** ** Typing inversion lemmas *)
+
+Lemma var_inversion Sigma Delta Gamma (x : var) A :
+  TY Sigma; Delta; Gamma |- ^x : A -> Gamma !! x = Some A.
+Proof. inversion 1; subst; auto. Qed.
+
+Lemma lam_inversion Sigma Delta Gamma e C :
+  TY Sigma; Delta; Gamma |- (lam: e) : C ->
+  exists A B, C = (A -> B)%ty /\ type_wf Delta A /\ TY Sigma; Delta; A :: Gamma |- e : B.
+Proof. inversion 1; subst; eauto 10. Qed.
+
+Lemma app_inversion Sigma Delta Gamma e1 e2 B :
+  TY Sigma; Delta; Gamma |- e1 e2 : B ->
+  exists A, TY Sigma; Delta; Gamma |- e1 : (A -> B) /\ TY Sigma; Delta; Gamma |- e2 : A.
+Proof. inversion 1; subst; eauto. Qed.
+
+Lemma if_inversion Sigma Delta Gamma e0 e1 e2 B :
+  TY Sigma; Delta; Gamma |- If e0 e1 e2 : B ->
+  TY Sigma; Delta; Gamma |- e0 : Bool /\
+  TY Sigma; Delta; Gamma |- e1 : B /\
+  TY Sigma; Delta; Gamma |- e2 : B.
+Proof. inversion 1; subst; eauto. Qed.
+
+Lemma binop_inversion Sigma Delta Gamma op e1 e2 B :
+  TY Sigma; Delta; Gamma |- BinOp op e1 e2 : B ->
+  exists A1 A2, bin_op_typed op A1 A2 B /\
+    TY Sigma; Delta; Gamma |- e1 : A1 /\ TY Sigma; Delta; Gamma |- e2 : A2.
+Proof. inversion 1; subst; eauto. Qed.
+
+Lemma type_app_inversion Sigma Delta Gamma e B :
+  TY Sigma; Delta; Gamma |- e <> : B ->
+  exists A C, B = A.[C/] /\ type_wf Delta C /\ TY Sigma; Delta; Gamma |- e : (forall: A).
+Proof. inversion 1; subst; eauto. Qed.
+
+Lemma type_lam_inversion Sigma Delta Gamma e B :
+  TY Sigma; Delta; Gamma |- (Lam: e) : B ->
+  exists A, B = (forall: A)%ty /\ TY upheap Sigma; (S Delta); upctx Gamma |- e : A.
+Proof. inversion 1; subst; eauto. Qed.
+
+Lemma type_pack_inversion Sigma Delta Gamma e B :
+  TY Sigma; Delta; Gamma |- (pack e) : B ->
+  exists A C, B = (exists: A)%ty /\ TY Sigma; Delta; Gamma |- e : (A.[C/])%ty /\ type_wf Delta C.
+Proof. inversion 1; subst; eauto 10. Qed.
+
+Lemma type_unpack_inversion Sigma Delta Gamma e e' B :
+  TY Sigma; Delta; Gamma |- (unpack e in e') : B ->
+  exists A, type_wf Delta B /\
+    TY Sigma; Delta; Gamma |- e : (exists: A) /\
+    TY upheap Sigma; S Delta; A :: (upctx Gamma) |- e' : (B.[ren (+1)]).
+Proof. inversion 1; subst; eauto 10. Qed.
+
+Lemma pair_inversion Sigma Delta Gamma e1 e2 C :
+  TY Sigma; Delta; Gamma |- (e1, e2) : C ->
+  exists A B, C = (A * B)%ty /\ TY Sigma; Delta; Gamma |- e1 : A /\ TY Sigma; Delta; Gamma |- e2 : B.
+Proof. inversion 1; subst; eauto. Qed.
+
+Lemma fst_inversion Sigma Delta Gamma e A :
+  TY Sigma; Delta; Gamma |- Fst e : A ->
+  exists B, TY Sigma; Delta; Gamma |- e : A * B.
+Proof. inversion 1; subst; eauto. Qed.
+
+Lemma snd_inversion Sigma Delta Gamma e B :
+  TY Sigma; Delta; Gamma |- Snd e : B ->
+  exists A, TY Sigma; Delta; Gamma |- e : A * B.
+Proof. inversion 1; subst; eauto. Qed.
+
+Lemma new_inversion Sigma Delta Gamma e B :
+  TY Sigma; Delta; Gamma |- (new e) : B ->
+  exists A, B = Ref A /\ TY Sigma; Delta; Gamma |- e : A.
+Proof. inversion 1; subst; eauto. Qed.
+
+Lemma load_inversion Sigma Delta Gamma e B:
+  TY Sigma; Delta; Gamma |- ! e : B ->
+  TY Sigma; Delta; Gamma |- e : Ref B.
+Proof. inversion 1; subst; eauto. Qed.
+
+Lemma store_inversion Sigma Delta Gamma e1 e2 B:
+  TY Sigma; Delta; Gamma |- (e1 <- e2) : B ->
+  TY Sigma; Delta; Gamma |- e1 : Ref B /\ TY Sigma; Delta; Gamma |- e2 : B.
+Proof. inversion 1; subst; eauto. Qed.
+
+(** ** Progress *)
+
+(** Canonical forms lemmas *)
+Lemma canonical_values_arr Sigma Delta Gamma e A B :
+  TY Sigma; Delta; Gamma |- e : (A -> B) ->
+  is_val e ->
+  exists e', e = (lam: e')%E.
+Proof.
+  inversion 1; simplify_eq; by eauto.
+Qed.
+
+Lemma canonical_values_forall Sigma Delta Gamma e A :
+  TY Sigma; Delta; Gamma |- e : (forall: A)%ty ->
+  is_val e ->
+  exists e', e = (Lam: e')%E.
+Proof.
+  inversion 1; simplify_eq; by eauto.
+Qed.
+
+Lemma canonical_values_exists Sigma Delta Gamma e A :
+  TY Sigma; Delta; Gamma |- e : (exists: A) ->
+  is_val e ->
+  exists e', e = (pack e')%E.
+Proof.
+  inversion 1; simplify_eq; by eauto.
+Qed.
+
+Lemma canonical_values_int Sigma Delta Gamma e :
+  TY Sigma; Delta; Gamma |- e : Int ->
+  is_val e ->
+  exists n: Z, e = (#n)%E.
+Proof.
+  inversion 1; simplify_eq; by eauto.
+Qed.
+
+Lemma canonical_values_bool Sigma Delta Gamma e :
+  TY Sigma; Delta; Gamma |- e : Bool ->
+  is_val e ->
+  exists b: bool, e = (#b)%E.
+Proof.
+  inversion 1; simplify_eq; by eauto.
+Qed.
+
+Lemma canonical_values_unit Sigma Delta Gamma e :
+  TY Sigma; Delta; Gamma |- e : Unit ->
+  is_val e ->
+  e = (#LitUnit)%E.
+Proof.
+  inversion 1; simplify_eq; by eauto.
+Qed.
+
+Lemma canonical_values_prod Sigma Delta Gamma e A B :
+  TY Sigma; Delta; Gamma |- e : A * B ->
+  is_val e ->
+  exists e1 e2, e = (e1, e2)%E /\ is_val e1 /\ is_val e2.
+Proof.
+  inversion 1; simplify_eq; by eauto 10.
+Qed.
+
+Lemma canonical_values_ref Sigma Delta Gamma e A:
+  TY Sigma; Delta; Gamma |- e : Ref A ->
+  is_val e ->
+  exists l: loc, e = (#l)%E /\ Sigma !! l = Some A.
+Proof.
+  inversion 1; simplify_eq; by eauto 10.
+Qed.
+
+Lemma type_progress Sigma h e A :
+  typed_heap Sigma h ->
+  TY Sigma; 0; [] |- e : A ->
+  progressive h e.
+Proof.
+  intros Hheap. remember [] as Gamma. remember 0 as n.
+  induction 1 as [| | Sigma Delta Gamma e1 e2 A B Hty IH1 _ IH2 | | Sigma Delta Gamma A B e Hty IH | Sigma Delta Gamma A B e Hwf Hty IH
+    | Sigma Delta Gamma A B e e' Hwf Hty1 IH1 Hty2 IH2 | | | | Sigma Delta Gamma e0 e1 e2 A Hty1 IH1 Hty2 IH2 Hty3 IH3
+    | Sigma Delta Gamma e1 e2 op A B C Hop Hty1 IH1 Hty2 IH2 | Sigma Delta Gamma e1 e2 A B Hty1 IH1 Hty2 IH2
+    | Sigma Delta Gamma e A B Hty IH | Sigma Delta Gamma e A B Hty IH
+    | Sigma Delta Gamma l A Hl | Sigma Delta Gamma e A Hty IH | Sigma Delta Gamma e1 e2 A Hty1 IH1 Hty2 IH2 | Sigma Delta Gamma e A Hty IH ].
+  - (* variable *) subst. by exfalso.
+  - (* lambda *) left. done.
+  - (* app *)
+    destruct (IH2 Hheap HeqGamma Heqn) as [H2|H2]; [destruct (IH1 Hheap HeqGamma Heqn) as [H1|H1]|].
+    + eapply canonical_values_arr in Hty as (e & ->); last done.
+      right. eexists _, _.
+      eapply base_contextual_step, BetaS; eauto.
+    + right. destruct H1 as (e1' & h' & Hstep). eauto.
+    + right. destruct H2 as (e2' & h' & ?). eauto.
+  - (* big lambda *) left. simpl. done.
+  - (* type app *)
+    right. destruct (IH Hheap HeqGamma Heqn) as [H1|H1].
+    + eapply canonical_values_forall in Hty as [e' ->]; last done.
+      eexists _, _. eapply base_contextual_step. econstructor.
+    + destruct H1 as (e' & h' & H1). eexists _, _. eapply contextual_step_tapp. done.
+  - (* pack *)
+    destruct (IH Hheap HeqGamma Heqn) as [H | H].
+    + left. done.
+    + right. destruct H as (e' & h' & H). eexists _, _.
+      eapply contextual_step_pack. done.
+  - (* unpack *)
+    destruct (IH1 Hheap HeqGamma Heqn) as [Hval | Hred].
+    + eapply canonical_values_exists in Hty1 as [e'' ->]; last done.
+      right. eexists _, _. eapply base_contextual_step. constructor; last done.
+      done.
+    + right. destruct Hred as (e'' & h'' & H). eexists _, _. eapply contextual_step_unpack. done.
+  - (* int *) left. done.
+  - (* bool *) left. done.
+  - (* unit *) left. done.
+  - (* if *)
+    destruct (IH1 Hheap HeqGamma Heqn) as [H1 | H1].
+    + eapply canonical_values_bool in Hty1 as (b & ->); last done.
+      right. destruct b; eexists _, _; eapply base_contextual_step; constructor.
+    + right. destruct H1 as (e0' & h' & Hstep).
+      eexists. eauto.
+  - (* binop *)
+    assert (A = Int /\ B = Int) as [-> ->].
+    { inversion Hop; subst A B C; done. }
+    destruct (IH2 Hheap HeqGamma Heqn) as [H2|H2]; [destruct (IH1 Hheap HeqGamma Heqn) as [H1|H1]|].
+    + right. eapply canonical_values_int in Hty1 as [n1 ->]; last done.
+      eapply canonical_values_int in Hty2 as [n2 ->]; last done.
+      inversion Hop; subst; simpl.
+      all: eexists _, _; eapply base_contextual_step; eapply BinOpS; eauto.
+    + right. destruct H1 as (e1' & h' & Hstep). eauto.
+    + right. destruct H2 as (e2' & h' & H2). eauto.
+  - (* pair *)
+    destruct (IH2 Hheap HeqGamma Heqn) as [H2|H2]; [destruct (IH1 Hheap HeqGamma Heqn) as [H1|H1]|].
+    + left. done.
+    + right. destruct H1 as (e1' & h' & Hstep). eauto.
+    + right. destruct H2 as (e2' & h' & H2). eauto.
+  - (* fst *)
+    destruct (IH Hheap HeqGamma Heqn) as [H | H].
+    + eapply canonical_values_prod in Hty as (e1 & e2 & -> & ? & ?); last done.
+      right. eexists _, _. eapply base_contextual_step. econstructor; done.
+    + right. destruct H as (e' & h' & H). eauto.
+  - (* snd *)
+    destruct (IH Hheap HeqGamma Heqn) as [H | H].
+    + eapply canonical_values_prod in Hty as (e1 & e2 & -> & ? & ?); last done.
+      right. eexists _, _. eapply base_contextual_step. econstructor; done.
+    + right. destruct H as (e' & h' & H). eauto.
+  - (* loc *)
+    by left.
+  - (* load *)
+    destruct (IH Hheap HeqGamma Heqn) as [Hval|Hred].
+    + eapply canonical_values_ref in Hty as (l & -> & Hlook); last done.
+      eapply Hheap in Hlook as (v & Hlook & Hty').
+      right. do 2 eexists. eapply base_contextual_step. by econstructor.
+    + right. destruct Hred as (e' & h' & Hred).
+      do 2 eexists. eauto.
+  - (* store *)
+    destruct (IH2 Hheap HeqGamma Heqn) as [H2|H2]; [destruct (IH1 Hheap HeqGamma Heqn) as [H1|H1]|].
+    + right. eapply canonical_values_ref in Hty1 as (l & -> & Hlook); last done.
+      eapply Hheap in Hlook as (v & Hlook & Hty').
+      apply is_val_rewrite in H2 as [v2 ->].
+      do 2 eexists. eapply base_contextual_step.
+      econstructor; rewrite ?to_of_val //.
+    + right. eapply is_val_rewrite in H2 as [v2 ->].
+      destruct H1 as (e1' & h' & Hstep). eauto 10.
+    + right. destruct H2 as (e2' & h' & H2). eauto.
+  - (* new *)
+    destruct (IH Hheap HeqGamma Heqn) as [Hval|Hred].
+    + right. eapply is_val_rewrite in Hval as [v ->].
+      do 2 eexists. eapply base_contextual_step.
+      econstructor; rewrite ?to_of_val //.
+    + right. destruct Hred as (e' & h' & Hred). eauto.
+Qed.
+
+(** ** Renamings and substitutions on types *)
+
+(** Well-formed type renamings from [Delta1] to [Delta2].
+(Or, equivalently: [Delta1] is included in [Delta2] via renaming [delta]. *)
+Definition wf_tren Delta1 Delta2 (delta : var -> var) :=
+  forall alpha, alpha < Delta1 -> delta alpha < Delta2.
+
+(** Renaming well-formedness is preserved when we increase both typing contexts
+by one and shift the renaming up. *)
+Lemma wf_tren_up delta Delta1 Delta2 :
+  wf_tren Delta1 Delta2 delta -> wf_tren (S Delta1) (S Delta2) (upren delta).
+Proof.
+  intros Hdelta [|k]; simpl; first by lia.
+  specialize (Hdelta k). lia.
+Qed.
+
+(** Type context [n] is included in [S n] with the successor renaming. **)
+Lemma wf_tren_S Delta :
+  wf_tren Delta (S Delta) S.
+Proof.
+  intros k. lia.
+Qed.
+
+(** Type well-formedness is preserved under renaming. *)
+Lemma type_wf_rename Delta1 Delta2 A delta :
+  wf_tren Delta1 Delta2 delta ->
+  type_wf Delta1 A ->
+  type_wf Delta2 (A.[ren delta]).
+Proof.
+  intros Hdelta. induction 1 in Delta2, Hdelta, delta |-*; asimpl; eauto.
+  - econstructor. eapply IHtype_wf, wf_tren_up. done.
+  - econstructor. eapply IHtype_wf, wf_tren_up. done.
+Qed.
+
+(** Well-formed type substitutions: [sigma] maps the types from context [Delta1]
+into types that are avlid in [Delta2]. *)
+Definition wf_tsubst Delta1 Delta2 sigma :=
+  forall alpha, alpha < Delta1 -> type_wf Delta2 (sigma alpha).
+
+(** On renamings, [wf_tren] and [wf_tsubst] are equivalent.
+(We don't actually need this lemma for the type safety proof, but it demonstrates
+that [wf_tsubst] is a generalization of [wf_tren].) *)
+Lemma wf_tsubst_tren Delta1 Delta2 (delta : var -> var) :
+  wf_tren Delta1 Delta2 delta <-> wf_tsubst Delta1 Delta2 (ren delta).
+Proof.
+  split.
+  - intros Hdelta k. specialize (Hdelta k). simpl. eauto with lia.
+  - intros Hdelta k Hk. specialize (Hdelta k Hk). by inversion Hdelta.
+Qed.
+
+Lemma wf_tsubst_up sigma Delta1 Delta2 :
+  wf_tsubst Delta1 Delta2 sigma -> wf_tsubst (S Delta1) (S Delta2) (up sigma).
+Proof.
+  intros Hdelta [|k]; asimpl.
+  - eauto with lia.
+  - specialize (Hdelta k). intros.
+    eapply type_wf_rename; last by eauto with lia.
+    eapply wf_tren_S.
+Qed.
+
+Lemma wf_tsubst_single Delta A :
+  type_wf Delta A ->
+  wf_tsubst (S Delta) Delta (A .: ids).
+Proof.
+  intros Hwf [|k] Hk; simpl.
+  - done.
+  - econstructor. lia.
+Qed.
+
+(** Applying a well-formed substitution preserves well-formedness. *)
+Lemma type_wf_substitution Delta1 Delta2 A sigma :
+  wf_tsubst Delta1 Delta2 sigma ->
+  type_wf Delta1 A ->
+  type_wf Delta2 A.[sigma].
+Proof.
+  intros Hsigma. induction 1 in Delta2, Hsigma, sigma |-*; simpl; eauto.
+  + econstructor; eapply IHtype_wf. eapply wf_tsubst_up. done.
+  + econstructor; eapply IHtype_wf. eapply wf_tsubst_up. done.
+Qed.
+
+(** Shifting of contexts and applying a substitution in a context commutes. *)
+Lemma upctx_subst sigma Gamma :
+  upctx (subst sigma <$> Gamma) = subst (up sigma) <$> upctx Gamma.
+Proof.
+  rewrite /upctx. apply list_eq. intros x. rewrite !list_lookup_fmap.
+  destruct (Gamma !! x) as [B|]; last done. by asimpl.
+Qed.
+
+Lemma upheap_subst sigma Sigma :
+  upheap (subst sigma <$> Sigma) = subst (up sigma) <$> upheap Sigma.
+Proof.
+  rewrite /upheap. apply map_eq. intros l. rewrite !lookup_fmap.
+  destruct (Sigma !! l) as [B|]; last done. by asimpl.
+Qed.
+
+(** Applying such a well-formed type substitution to a typing judgment (both the
+context and the result type) preserves typing. *)
+Lemma type_tsubstitution Sigma Delta1 Delta2 Gamma e A sigma :
+  wf_tsubst Delta1 Delta2 sigma ->
+  TY Sigma; Delta1; Gamma |- e : A ->
+  TY (subst sigma) <$> Sigma; Delta2; (subst sigma) <$> Gamma |- e : A.[sigma].
+Proof.
+  intros Hsigma.
+  induction 1 as [ Sigma Delta Gamma x A Heq| | | Sigma Delta Gamma e A Hty IH | |Sigma Delta Gamma A B e Hwf Hty IH
+    |Sigma Delta Gamma A B e e' Hwf Hty1 IH1 Hty2 IH2 | | | | |? ? ? ? ? ? ? ? ? Hop | | | | | | |]
+    in Hsigma, sigma, Delta2 |-*; simpl.
+  - (* var *) econstructor. rewrite list_lookup_fmap Heq //=.
+  - (* lam *) econstructor; last by eapply type_wf_substitution.
+    rewrite -fmap_cons. eauto.
+  - (* app *) eauto.
+  - (* tlam *) econstructor. rewrite upctx_subst upheap_subst.
+    eapply IH. eapply wf_tsubst_up. done.
+  - (* tapp *) replace (A.[B/].[sigma]) with (A.[up sigma].[B.[sigma]/]) by by asimpl.
+    eauto using type_wf_substitution.
+  - (* pack *)
+    eapply (type_pack _ _ _ _ (subst sigma B)).
+    + eapply type_wf_substitution; done.
+    + replace (A.[up sigma].[B.[sigma]/]) with (A.[B/].[sigma]) by by asimpl.
+      eauto using type_wf_substitution.
+  - (* unpack *)
+    eapply (type_unpack _ _ _ A.[up sigma]).
+    + eapply type_wf_substitution; done.
+    + replace (exists: A.[up sigma])%ty with ((exists: A).[sigma])%ty by by asimpl.
+      eapply IH1. done.
+    + rewrite upctx_subst upheap_subst. rewrite -fmap_cons.
+      replace (B.[sigma].[ren (+1)]) with (B.[ren(+1)].[up sigma]) by by asimpl.
+      eapply IH2. eapply wf_tsubst_up. done.
+  - (* int *) eauto.
+  - (* bool *) eauto.
+  - (* unit *) eauto.
+  - (* if *) eauto.
+  - (* binop *) inversion Hop; subst; eauto.
+  - (* pair *) eauto.
+  - (* fst *) eauto.
+  - (* snd *) eauto.
+  - (* loc *) econstructor. rewrite lookup_fmap H //=.
+  - (* load *) eauto.
+  - (* store *) eauto.
+  - (* new *) eauto.
+Qed.
+
+(** We can derive the on-paper version by specializing to single substitution.
+
+We also make the lemma easier to apply by introducing [Gamma'] which must
+be equal to [Gamma] with the substitution applied everywhere.
+This means we can [eapply] the lemma and then prove the equality, rather than
+having to get things into the right shape for [eapply] to even work.
+The same goes for [A'] *)
+Lemma type_tsubstitution_single Sigma Sigma' Delta Gamma Gamma' e A A' B :
+  type_wf Delta B ->
+  TY Sigma; (S Delta); Gamma |- e : A ->
+  Sigma' = (fun A' => A'.[B/]) <$> Sigma ->
+  Gamma' = (fun A' => A'.[B/]) <$> Gamma ->
+  A' = A.[B/] ->
+  TY Sigma'; Delta; Gamma' |- e : A'.
+Proof.
+  intros HB He -> -> ->. eapply type_tsubstitution; last done.
+  eapply wf_tsubst_single. done.
+Qed.
+
+(** ** Renamings and substitutions on terms *)
+
+(** Type-preserving renamings ("context inclusion") *)
+Definition typed_ren (Gamma1 Gamma2 : typing_context) (delta : var -> var) :=
+  forall x B, Gamma1 !! x = Some B -> Gamma2 !! (delta x) = Some B.
+
+(** As before, [typed_ren] is preserved if we add the same type at index 0 in
+both contexts. *)
+Lemma typed_ren_up delta Gamma1 Gamma2 A :
+  typed_ren Gamma1 Gamma2 delta -> typed_ren (A :: Gamma1) (A :: Gamma2) (upren delta).
+Proof.
+  intros Hsigma [|x] C; simpl; first done. eauto.
+Qed.
+
+(** [Gamma] is included in [A :: Gamma] with the successor renaming. *)
+Lemma typed_ren_S A Gamma :
+  typed_ren Gamma (A :: Gamma) S.
+Proof.
+  intros x C. eauto.
+Qed.
+
+(** We also get a new preservation lemma for renaming the contexts themselves using [upctx]. *)
+Lemma typed_ren_upctx delta Gamma1 Gamma2 :
+  typed_ren Gamma1 Gamma2 delta -> typed_ren (upctx Gamma1) (upctx Gamma2) delta.
+Proof.
+  intros Hsigma x C. rewrite !list_lookup_fmap.
+  intros (C' & ? & ->)%fmap_Some. eapply fmap_Some. eauto.
+Qed.
+
+(** Then we get to weakening, or the "renaming" lemma. *)
+Lemma type_renaming delta Sigma Delta Gamma1 Gamma2 e A :
+  typed_ren Gamma1 Gamma2 delta ->
+  TY Sigma; Delta; Gamma1 |- e : A ->
+  TY Sigma; Delta; Gamma2 |- e.[ren delta] : A.
+Proof.
+  intros Hsigma. induction 1 in Gamma2, delta, Hsigma.
+  (* That's a lot of cases. Fortunately, most of them are trivial since they
+  don't do anything with binders. *)
+  all: asimpl; eauto.
+  (* The remaining 3 cases have to be done by hand. *)
+  - (* lam *) constructor; last done.
+    eapply IHsyn_typed, typed_ren_up. done.
+  - (* tlam *) econstructor. eapply IHsyn_typed.
+    eapply typed_ren_upctx. done.
+  - (* unpack *) econstructor.
+    + done.
+    + eapply IHsyn_typed1. done.
+    + eapply IHsyn_typed2. eapply typed_ren_up, typed_ren_upctx. done.
+Qed.
+
+(** Type-preserving substitution *)
+Definition typed_subst Sigma Delta Gamma1 Gamma2 (sigma : var -> expr) :=
+  forall x B, Gamma1 !! x = Some B -> TY Sigma; Delta; Gamma2 |- sigma x : B.
+
+(** On renamings, [typed_ren] and [typed_subst] are equivalent.
+(We don't actually need this lemma for the type safety proof, but it demonstrates
+that [typed_subst] is a generalization of [typed_ren].) *)
+Lemma typed_subst_ren Sigma Delta (Gamma1 Gamma2 : typing_context) (delta : var -> var) :
+  typed_ren Gamma1 Gamma2 delta <-> typed_subst Sigma Delta Gamma1 Gamma2 (ren delta).
+Proof.
+  split.
+  - intros Hdelta x B Hx. specialize (Hdelta _ _ Hx). by constructor.
+  - intros Hdelta x B Hx. specialize (Hdelta _ _ Hx). by inversion Hdelta.
+Qed.
+
+(** As always, we can extend the context with a new type if we also shift the
+substitution. *)
+Lemma typed_subst_up Sigma Delta sigma Gamma1 Gamma2 A :
+  typed_subst Sigma Delta Gamma1 Gamma2 sigma ->
+  typed_subst Sigma Delta (A :: Gamma1) (A :: Gamma2) (up sigma).
+Proof.
+  intros Hsigma [|x] C; simpl; intros.
+  - simplify_eq. constructor. done.
+  - asimpl. eapply type_renaming; last by eauto. eapply typed_ren_S.
+Qed.
+
+(** We can remove a single type from the context if the substitution puts in a
+well-typed term. *)
+Lemma typed_subst_single Sigma Delta Gamma A e :
+  TY Sigma; Delta; Gamma |- e : A ->
+  typed_subst Sigma Delta (A :: Gamma) Gamma (e .: ids).
+Proof.
+  intros He [|x] C; simpl; intros Hx.
+  - simplify_eq. done.
+  - eauto.
+Qed.
+
+(** And [typed_subst] is preserved when we shift up the typing context by 1. *)
+Lemma typed_subst_upctx Sigma Delta sigma Gamma1 Gamma2 :
+  typed_subst Sigma Delta Gamma1 Gamma2 sigma ->
+  typed_subst (upheap Sigma) (S Delta) (upctx Gamma1) (upctx Gamma2) sigma.
+Proof.
+  intros Hsigma x C. rewrite !list_lookup_fmap.
+  intros (C' & ? & ->)%fmap_Some. eapply type_tsubstitution; last by eauto.
+  eapply wf_tsubst_tren, wf_tren_S.
+Qed.
+
+(** Finally, the main substitution lemma *)
+Lemma type_substitution sigma Sigma Delta e Gamma1 Gamma2 A :
+  typed_subst Sigma Delta Gamma1 Gamma2 sigma ->
+  TY Sigma; Delta; Gamma1 |- e : A ->
+  TY Sigma; Delta; Gamma2 |- e.[sigma] : A.
+Proof.
+  intros Hsigma. induction e in Sigma, Delta, Gamma1, Gamma2, A, sigma, Hsigma |- *.
+  - (* var *) intros Hp % var_inversion.
+    specialize (Hsigma _ _ Hp). asimpl. done.
+  - (* lam *) intros (C & D & -> & Hwf & Hty)%lam_inversion. asimpl.
+    econstructor; last done. eapply IHe; last done. by eapply typed_subst_up.
+  - (* app *) intros (C & Hty1 & Hty2) % app_inversion. asimpl. eauto.
+  - (* literals *) asimpl. inversion 1; subst; auto.
+  - (* binop *) intros (? & ? & Hop & H1 & H2) % binop_inversion. asimpl.
+    destruct op; inversion Hop; subst; eauto.
+  - (* if *) intros (H1 & H2 & H3)%if_inversion. asimpl. eauto.
+  - (* tapp *) intros (C & D & -> & Hwf & Hty) % type_app_inversion. asimpl. eauto.
+  - (* tlam *) intros (C & -> & Hty)%type_lam_inversion. asimpl. econstructor.
+    eapply IHe; last done. eapply typed_subst_upctx. done.
+  - (* pack *) intros (C & D & -> & Hty & Hwf)%type_pack_inversion.
+    econstructor; [done..|]. eapply IHe; done.
+  - (* unpack *) intros (C & Hwf & Hty1 & Hty2)%type_unpack_inversion. asimpl.
+    econstructor; first done.
+    + eapply IHe; done.
+    + eapply IHe0; last done.
+      eapply typed_subst_up, typed_subst_upctx. done.
+  - (* pair *) intros (? & ? & -> & ? & ?) % pair_inversion. asimpl. eauto.
+  - (* fst *) intros (? & ?)%fst_inversion. asimpl. eauto.
+  - (* snd *) intros (? & ?)%snd_inversion. asimpl. eauto.
+  - (* load *) intros Hty % load_inversion. asimpl. eauto.
+  - (* store *) intros (Hty1 & Hty2)% store_inversion. asimpl. eauto.
+  - (* new *) intros (C & -> & Hty) % new_inversion. asimpl. eauto.
+Qed.
+
+(** We can derive the on-paper version by specializing to single substitution. *)
+Lemma type_substitution_single e e' Sigma Delta Gamma A B :
+  TY Sigma; Delta; Gamma |- e' : B ->
+  TY Sigma; Delta; B :: Gamma |- e : A ->
+  TY Sigma; Delta; Gamma |- e.[e'/] : A.
+Proof.
+  intros. eapply type_substitution; last done.
+  eapply typed_subst_single. done.
+Qed.
+
+(** ** Preservation *)
+
+(** Heap typing lemmas *)
+Lemma heap_subseteq_insert h l A Sigma:
+  typed_heap Sigma h -> h !! l = None -> Sigma `subseteq` <[l:=A]> Sigma.
+Proof.
+  intros Hheap Hlook. eapply insert_subseteq.
+  specialize (Hheap l). destruct (lookup) as [B|]; last done.
+  specialize (Hheap B eq_refl) as (w & Hsome & _). congruence.
+Qed.
+
+Lemma heap_subseteq_upheap Sigma1 Sigma2 :
+  Sigma1 `subseteq` Sigma2 ->
+  upheap Sigma1 `subseteq` upheap Sigma2.
+Proof. apply map_fmap_mono. Qed.
+
+Lemma type_heap_subseteq Sigma1 Sigma2 Delta Gamma e A :
+  TY Sigma1; Delta; Gamma |- e : A ->
+  Sigma1 `subseteq` Sigma2 ->
+  TY Sigma2; Delta; Gamma |- e : A.
+Proof.
+  induction 1 in Sigma2 |- *; eauto using heap_subseteq_upheap.
+  (* Most typing rules are handled automatically. Only location typing remains. *)
+  - (* loc *) constructor. eapply lookup_weaken; eauto.
+Qed.
+
+Lemma typed_heap_insert h Sigma e v l B :
+  typed_heap Sigma h ->
+  h !! l = None ->
+  TY Sigma; 0; [] |- e : B ->
+  to_val e = Some v ->
+  typed_heap (<[l:=B]> Sigma) (<[l:=v]> h).
+Proof.
+  intros Hheap Hlook Hty Hval l' A. rewrite lookup_insert_Some.
+  intros [(-> & ->)|(Hne & Hlook')].
+  - exists v. split; first eapply lookup_insert_eq.
+    eapply of_to_val in Hval as ->.
+    eapply type_heap_subseteq; first eapply Hty.
+    by eapply heap_subseteq_insert.
+  - eapply Hheap in Hlook' as (w & Hlook' & Hty').
+    eexists; split.
+    + rewrite lookup_insert_ne //=.
+    + eapply type_heap_subseteq; first eapply Hty'.
+      by eapply heap_subseteq_insert.
+Qed.
+
+Lemma typed_heap_update h Sigma e v l B :
+  typed_heap Sigma h ->
+  Sigma !! l = Some B ->
+  TY Sigma; 0; [] |- e : B ->
+  to_val e = Some v ->
+  typed_heap Sigma (<[l:=v]> h).
+Proof.
+  intros Hheap Hlook Hty Hval l' A Hlook'.
+  eapply Hheap in Hlook' as Hlook''.
+  destruct Hlook'' as (w & Hold & Hval').
+  destruct (decide (l = l')); subst.
+  - exists v. split; first eapply lookup_insert_eq.
+    eapply of_to_val in Hval as ->.
+    rewrite Hlook in Hlook'. by injection Hlook' as ->.
+  - rewrite lookup_insert_ne //=. eauto.
+Qed.
+
+Lemma upheap_subst_single Sigma A :
+  (λ B : type, B.[A/]) <$> upheap Sigma = Sigma.
+Proof.
+  rewrite /upheap -map_fmap_compose. apply map_eq.
+  intros l. rewrite lookup_fmap. destruct (Sigma !! l) as [v|]; last done.
+  simpl. f_equal. asimpl. done.
+Qed.
+
+(** Base step preservation **)
+Lemma type_preservation_base_step Sigma e h e' h' A :
+  TY Sigma; 0; [] |- e : A ->
+  typed_heap Sigma h ->
+  base_step (h, e) (h', e') ->
+  exists Sigma',
+    Sigma `subseteq` Sigma' /\
+    typed_heap Sigma' h' /\
+    TY Sigma'; 0; [] |- e' : A.
+Proof.
+  intros Hty Hheap Hstep.
+  inversion Hstep; subst.
+  - (* beta *) eapply app_inversion in Hty as (B & Hlam &?).
+    eapply lam_inversion in Hlam as (C & D & Heq & Hwf & Hty).
+    simplify_eq.
+    eexists. split; first reflexivity. split; first done.
+    eapply type_substitution_single; done.
+  - (* tbeta *)
+    eapply type_app_inversion in Hty as (B & C & -> & Hwf & Hty).
+    eapply type_lam_inversion in Hty as (A & Heq & Hty).
+    simplify_eq.
+    eexists. split; first reflexivity. split; first done.
+    eapply type_tsubstitution_single; eauto using upheap_subst_single.
+  - (* unpack *)
+    eapply type_unpack_inversion in Hty as (B & Hwf & Hty1 & Hty2).
+    eapply type_pack_inversion in Hty1 as (B' & C & [= <-] & Hty1 & ?).
+    eexists. split; first reflexivity. split; first done.
+    eapply type_substitution_single.
+    { done. }
+    eapply type_tsubstitution_single; [eauto using upheap_subst_single..|].
+    asimpl. done.
+  - (* binop *)
+    eapply binop_inversion in Hty as (A1 & A2 & Hop & Hty1 & Hty2).
+    assert (A1 = Int /\ A2 = Int /\ (A = Int \/ A = Bool)) as (-> & -> & HC).
+    { inversion Hop; subst; eauto. }
+    eapply canonical_values_int in Hty1 as [n ->]; last by eauto.
+    eapply canonical_values_int in Hty2 as [m ->]; last by eauto.
+    simplify_eq/=.
+    eexists. split; first reflexivity. split; first done.
+    inversion Hop; subst; simpl in *; simplify_eq; constructor.
+  - (* if true *) eapply if_inversion in Hty as (H1 & H2 & H3).
+    eexists. split; first reflexivity. split; first done.
+    done.
+  - (* if false *) eapply if_inversion in Hty as (H1 & H2 & H3).
+    eexists. split; first reflexivity. split; first done.
+    done.
+  - (* fst *) eapply fst_inversion in Hty as (B & (? & ? & [= <- <-] & ? & ?)%pair_inversion).
+    eexists. split; first reflexivity. split; first done.
+    done.
+  - (* snd *) eapply snd_inversion in Hty as (B & (? & ? & [= <- <-] & ? & ?)%pair_inversion).
+    eexists. split; first reflexivity. split; first done.
+    done.
+  - (* new *) eapply new_inversion in Hty as (B & -> & Hty).
+    set (l := fresh (dom h)).
+    exists (<[l := B]> Sigma).
+    assert (h !! l = None).
+    { apply not_elem_of_dom. apply is_fresh. }
+    split; first by eapply heap_subseteq_insert. split.
+    + by eapply typed_heap_insert.
+    + econstructor. rewrite lookup_insert_eq. done.
+  - (* load *) eapply load_inversion in Hty.
+    eexists. split; first reflexivity. split; first done.
+    eapply canonical_values_ref in Hty as (l' & Heq & Hlook); last done.
+    simplify_eq. eapply Hheap in Hlook as (w & Hlook & Hty).
+    simplify_eq. done.
+  - (* store *) eapply store_inversion in Hty as (Hty1 & Hty2).
+    eexists. split; first reflexivity. split.
+    + eapply canonical_values_ref in Hty1 as (l' & Heq & Hlook); last done.
+      simplify_eq. eapply typed_heap_update; done.
+    + done.
+Qed.
+
+(** Evaluation context typing *)
+Definition typed_ectx Sigma (K: ectx) (A B: type) :=
+  forall Sigma' e,
+    Sigma `subseteq` Sigma' ->
+    TY Sigma'; 0; [] |- e : A ->
+    TY Sigma'; 0; [] |- (fill K e) : B.
+
+Lemma fill_typing_decompose Sigma K e A :
+  TY Sigma; 0; [] |- fill K e : A ->
+  exists B, TY Sigma; 0; [] |- e : B /\ typed_ectx Sigma K B A.
+Proof.
+  unfold typed_ectx; induction K in A |-*; simpl; inversion 1; subst; eauto.
+  all: edestruct IHK as (? & ? & ?); eauto 10 using type_heap_subseteq, heap_subseteq_upheap.
+Qed.
+
+Lemma fill_typing_compose Sigma K e A B :
+  TY Sigma; 0; [] |- e : B ->
+  typed_ectx Sigma K B A ->
+  TY Sigma; 0; [] |- fill K e : A.
+Proof.
+  intros H1 H2; by eapply H2.
+Qed.
+
+Lemma typed_ectx_heap_subseteq Sigma1 Sigma2 K A B :
+  typed_ectx Sigma1 K A B ->
+  Sigma1 `subseteq` Sigma2 ->
+  typed_ectx Sigma2 K A B.
+Proof.
+  intros Hectx HSigma ??? Hty. eapply Hectx; last done.
+  by etrans.
+Qed.
+
+(** Presevration lemma *)
+Lemma type_preservation {Sigma h e h' e' A} :
+  TY Sigma; 0; [] |- e : A ->
+  typed_heap Sigma h ->
+  contextual_step (h, e) (h', e') ->
+  exists Sigma',
+    Sigma `subseteq` Sigma' /\
+    typed_heap Sigma' h' /\
+    TY Sigma'; 0; [] |- e' : A.
+Proof.
+  intros Hty Hheap Hstep. inversion Hstep as [K e1 e2 ? ? ? ? ? ? Hbstep].
+  simplify_eq.
+  eapply fill_typing_decompose in Hty as [B [Hty ?]].
+  eapply type_preservation_base_step in Hty as (Sigma' & Hincl & Hheap' & Hty'); [|done..].
+  eexists. split; first done. split; first done.
+  eapply fill_typing_compose; eauto using typed_ectx_heap_subseteq.
+Qed.
+
+(** Top-level type safety theorem. *)
+
+Theorem type_safety e A :
+  TY empty; 0; [] |- e : A ->
+  forall h, safe h e.
+Proof.
+  intros Hty h.
+  remember empty as Sigma.
+  assert (typed_heap Sigma h) as Hheap.
+  { intros ??. rewrite HeqSigma lookup_empty. done. }
+  clear HeqSigma.
+  intros h' e'.
+  remember (h, e) as cfg. remember (h', e') as cfg'.
+  induction 1 as [|?[??]? Hstep Hsteps IH] in h', e', Heqcfg', Sigma, h, e, Heqcfg, Hty, Hheap |- *; simplify_eq.
+  - eapply type_progress; done.
+  - destruct (type_preservation Hty Hheap Hstep) as (Sigma' & ? & ? & ?).
+    eapply (IH _ Sigma'); eauto.
+Qed.
